Identare + functie pentru adaugarea valorii pe un index indicat
Am creat o functie method care se asigura ca valoarea adaugata se adauga respectand validitatea si corectitudinea solutiei

Problema_Bancnotelor.dfy
@@ -1,312 +1,317 @@
-function method power(A:int, N:nat):int
+function method power(A: int, N: nat): int 
 {
-	if (N==0) then 1 else A * power(A,N-1)
+  if (N == 0) then 1
+  else A * power(A, N - 1)
 }
 
-method pow(A:int, N:int) returns (x:int)
-	requires N >= 0
-	ensures x == power(A, N)
+method pow(A: int, N: int) returns(x: int)
+  requires N >= 0
+  ensures x == power(A, N) 
 {
-	x := 1;
-	var i := N;
+  x:= 1;
+  var i:= N;
 
-	while i != 0
-		invariant x == power(A, (N-i))
-	{ 
-		x := x * A;
-		i := i - 1;
-	}
-} 
+  while i != 0
+  invariant x == power(A, (N - i)) 
+  {
+    x:= x * A;
+    i:= i - 1;
+  }
+}
 
-predicate hasSixElem(solution: seq<int>)
+predicate hasSixElem(solution: seq < int > ) 
 {
   |solution| == 6
 }
 
-predicate isValidSolution (solution: seq<int>)
+predicate isValidSolution(solution: seq < int > ) 
 {
-    hasSixElem(solution) && solution[0] >= 0 && solution[1] >= 0 && solution[2] >= 0 && solution[3] >=0 && solution[4] >=0 && solution[5] >=0
+  hasSixElem(solution) && solution[0] >= 0 && solution[1] >= 0 && solution[2] >= 0 && solution[3] >= 0 && solution[4] >= 0 && solution[5] >= 0
 }
 
-function method solutionsSum(banknote1: seq<int>, banknote2: seq<int>): seq<int>
+function method solutionsSum(banknote1: seq < int > , banknote2: seq < int > ): seq < int >
   requires hasSixElem(banknote1)
-  requires hasSixElem(banknote2)
+  requires hasSixElem(banknote2) 
 {
-  [banknote1[0] + banknote2[0], banknote1[1] + banknote2[1], banknote1[2] + banknote2[2], 
-  banknote1[3] + banknote2[3], banknote1[4] + banknote2[4],banknote1[5] + banknote2[5]]
+  [banknote1[0] + banknote2[0], banknote1[1] + banknote2[1], banknote1[2] + banknote2[2],
+    banknote1[3] + banknote2[3], banknote1[4] + banknote2[4], banknote1[5] + banknote2[5]]
 }
 
-function solutionElementsSum(solution: seq<int>): int
-  requires hasSixElem(solution)
+function solutionElementsSum(solution: seq < int > ): int
+  requires hasSixElem(solution) 
 {
-  solution[0]*1 + solution[1]*2 + solution[2]*4 + solution[3]*8 + solution[4]*16 + solution[5]*32
+  solution[0] * 1 + solution[1] * 2 + solution[2] * 4 + solution[3] * 8 + solution[4] * 16 + solution[5] * 32
 }
 
-predicate isSolution(solution: seq<int>, sum: int)
-  requires isValidSolution(solution)
+predicate isSolution(solution: seq < int > , sum: int)
+  requires isValidSolution(solution) 
 {
-   solutionElementsSum(solution) == sum 
+  solutionElementsSum(solution) == sum
 }
 
-function cost(solution: seq<int>): int
-  requires isValidSolution(solution)
+function cost(solution: seq < int >): int
+  requires isValidSolution(solution) 
 {
   solution[0] + solution[1] + solution[2] + solution[3] + solution[4] + solution[5]
 }
 
-predicate isOptimalSolution(solution: seq<int>, sum: int)
-  requires isValidSolution(solution)
+predicate isOptimalSolution(solution: seq < int > , sum: int)
+  requires isValidSolution(solution) 
 {
   isSolution(solution, sum) &&
-  forall possibleSolution :: isValidSolution(possibleSolution) && isSolution(possibleSolution,sum)  ==> cost(possibleSolution) >= cost(solution)
+    forall possibleSolution::isValidSolution(possibleSolution) && isSolution(possibleSolution, sum) ==> cost(possibleSolution) >= cost(solution)
 }
 
-predicate addOptimRestEqualsOptimSum(rest: int, sum: int, x: seq<int>)
-  requires isValidSolution(x)
+predicate addOptimRestEqualsOptimSum(rest: int, sum: int, x: seq < int >)
+  requires isValidSolution(x) 
 {
   /* addOptimRestEqualsOptimSum(rest, sum, x) x is a valid solution for sum-rest, let's supose y is a valid solution ;
   if y is a solution for rest then x+y is a solution for sum 
   if y optimal for rest then x+y optimal for sum */
 
-  forall y :: isValidSolution(y)==>
-        (isSolution(y,rest) ==>
-        isSolution(solutionsSum(y,x), sum))
-        &&
-        ( isOptimalSolution(y,rest) ==>
-          isOptimalSolution(solutionsSum(y,x), sum))
+  forall y::isValidSolution(y) ==>
+    (isSolution(y, rest) ==>
+      isSolution(solutionsSum(y, x), sum)) &&
+    (isOptimalSolution(y, rest) ==>
+      isOptimalSolution(solutionsSum(y, x), sum))
 
 }
 
 method maxBanknote(sum: int) returns(index: int)
   requires sum > 0
-  ensures 0 <= index <=5
-  ensures 0 <= power(2,index) <= sum
-  ensures (index!=5 &&  power(2,index+1) > sum) || index==5
+  ensures 0 <= index <= 5
+  ensures 0 <= power(2, index) <= sum
+  ensures(index != 5 && power(2, index + 1) > sum) || index == 5 
 {
-  index:=5;
-  if(power(2,index)>sum)
+  index:= 5;
+  if (power(2, index) > sum) 
   {
-    assert power(2,index+1)>sum;
-     while( power(2,index)>sum && index > 0)
-      invariant power(2,index+1)>sum
-    {
-      index:=index-1;
-      assert power(2,index+1)>sum;
-    }
-  }
-  else
+    assert power(2, index + 1) > sum;
+    while (power(2, index) > sum && index > 0)
+      invariant power(2, index + 1) > sum 
+      {
+        index:= index - 1;
+        assert power(2, index + 1) > sum;
+      }
+  } 
+    else 
   {
     //we know the index is 5
-    assert index==5;
+    assert index == 5;
   }
 }
 
-lemma exchangeArgument(rest: int, currentSolution: seq<int>, index: int)
-    requires 0 <= index <= 4
-    requires power(2,index) <= rest < power(2,index+1) 
-    requires isValidSolution(currentSolution)
-    requires isOptimalSolution(currentSolution, rest - power(2,index))
-    ensures isOptimalSolution(currentSolution[index:=currentSolution[index]+1], rest)
+function method addValueToIndex(solution: seq<int>, value: int, index: int): seq<int>
+  requires 0 <= index <= 5
+  requires isValidSolution(solution)
+  requires solution[index] + value >= 0
+  ensures isValidSolution(solution)
+  ensures solutionElementsSum(solution) + value*power(2, index) == solutionElementsSum(solution[index:=solution[index]+value])
 {
-      var banknote:=power(2,index);
-      var solution := currentSolution[index:=currentSolution[index]+1];
-      assert isSolution(solution, rest);
-      var i:=index;
-      if(!isOptimalSolution(solution, rest))
+  solution[index:= solution[index] + value]
+}
+
+lemma exchangeArgument(rest: int, currentSolution: seq < int > , index: int)
+  requires 0 <= index <= 4
+  requires power(2, index) <= rest < power(2, index + 1)
+  requires isValidSolution(currentSolution)
+  requires isOptimalSolution(currentSolution, rest - power(2, index))
+  ensures isOptimalSolution(currentSolution[index:= currentSolution[index] + 1], rest) 
+{
+    var banknote:= power(2, index);
+    var solution:= currentSolution[index:= currentSolution[index] + 1];
+    assert isValidSolution(solution);
+    assert isSolution(solution, rest);
+    var i:= index;
+    if (!isOptimalSolution(solution, rest)) 
     {
-        
-      var optimalSolution :| isValidSolution(optimalSolution) && isSolution(optimalSolution, rest) &&
-      isOptimalSolution(optimalSolution, rest) && cost(optimalSolution) < cost(solution);
+      var optimalSolution:| isValidSolution(optimalSolution) && isSolution(optimalSolution, rest) &&
+        isOptimalSolution(optimalSolution, rest) && cost(optimalSolution) < cost(solution);
 
       assert cost(solution) == cost(currentSolution) + 1;
       assert isOptimalSolution(optimalSolution, rest);
 
-       if(optimalSolution[index] >= 1)
+      if (optimalSolution[index] -1 >= 0) 
       {
-          var betterSolution := optimalSolution[i:=optimalSolution[i]-1];
-          assert isSolution(betterSolution, rest - banknote);
-          assert cost(betterSolution) == cost(optimalSolution) - 1;
-          assert cost(optimalSolution) - 1 < cost(currentSolution);
-          assert false;
-      }
-      else
-      { 
-        while ( 0 < i )
-        invariant  0 <= i <= index
-        invariant forall x :: index >= x >= i ==> optimalSolution[x] <= 1
+        assert optimalSolution[index]-1 >= 0;
+        var betterSolution:= addValueToIndex(optimalSolution,-1,index);
+        assert isSolution(betterSolution, rest - banknote);
+        assert cost(betterSolution) == cost(optimalSolution) - 1;
+        assert cost(optimalSolution) - 1 < cost(currentSolution);
+        assert false;
+      } 
+      else 
+      {
+        while (0 < i)
+          invariant 0 <= i <= index
+          invariant forall x::index >= x >= i ==> optimalSolution[x] <= 1 
         {
-            i:= i - 1;
-            assert isOptimalSolution(optimalSolution, rest);
-            if(optimalSolution[i] > 1)
-            {
-              var optimalSolution' := optimalSolution[i:=optimalSolution[i]-2];
-              optimalSolution' := optimalSolution'[i+1:=optimalSolution'[i+1]+1];
-              assert isSolution(optimalSolution', rest);
-              assert cost(optimalSolution') == cost(optimalSolution) - 1;
-              assert cost(optimalSolution') < cost(optimalSolution);
-              assert false;
-          }   
+          i:= i - 1;
+          assert isOptimalSolution(optimalSolution, rest);
+          if (optimalSolution[i] > 1) 
+          {
+            var optimalSolution' := optimalSolution[i:=optimalSolution[i]-2];
+            optimalSolution' := optimalSolution' [i + 1:= optimalSolution'[i+1]+1];
+            assert isSolution(optimalSolution', rest);
+            assert cost(optimalSolution') == cost(optimalSolution) - 1;
+            assert cost(optimalSolution') < cost(optimalSolution);
+            assert false;
+          }
         }
-        assert solutionElementsSum(optimalSolution) <= banknote -1;
-        assert rest >= banknote;
-        assert solutionElementsSum(optimalSolution) <= rest-1;
-        assert isOptimalSolution(optimalSolution, rest);
-        assert false; 
+        assert solutionElementsSum(optimalSolution) <= banknote - 1; assert rest >= banknote; assert solutionElementsSum(optimalSolution) <= rest - 1; assert isOptimalSolution(optimalSolution, rest); assert false;
       }
     }
-}
+  }
 
-lemma exchangeArgument32(rest: int, sum: int, currentSolution: seq<int>, optimalSolution:seq<int>)
-    requires 32 <= rest 
-    requires isValidSolution(optimalSolution)
-    requires isOptimalSolution(optimalSolution, rest - 32)
-    ensures isOptimalSolution(optimalSolution[5:=optimalSolution[5]+1], rest)
+lemma exchangeArgument32(rest: int, sum: int, currentSolution: seq < int > , optimalSolution: seq < int > )
+  requires 32 <= rest
+  requires isValidSolution(optimalSolution)
+  requires isOptimalSolution(optimalSolution, rest - 32)
+  ensures isOptimalSolution(optimalSolution[5:= optimalSolution[5] + 1], rest) 
 {
-  var solution := optimalSolution[5:=optimalSolution[5]+1]; 
-  var i := 4;
-  if(!isOptimalSolution(solution, rest))
-  { 
+  var solution:= optimalSolution[5:= optimalSolution[5] + 1];
+  var i:= 4;
+  if (!isOptimalSolution(solution, rest)) 
+  {
     //if we have 2 of i is optimal to have an 32 so we don't have 2 of 16
-    if(optimalSolution[i] > 1)
-    { 
-      var solution := optimalSolution[i:=optimalSolution[i]-2];
-          solution :=solution[i+1:=solution[i+1]+1];
-          assert isSolution(solution, rest - 32);
-          assert cost(solution) == cost(optimalSolution) - 1;
-          assert cost(optimalSolution) - 1 < cost(solution);
-          assert false;
-    }
+    if (optimalSolution[i] > 1) 
+    {
+      var solution:= optimalSolution[i:= optimalSolution[i] - 2];
+      solution:= solution[i + 1:= solution[i + 1] + 1];
+      assert isSolution(solution, rest - 32);
+      assert cost(solution) == cost(optimalSolution) - 1;
+      assert cost(optimalSolution) - 1 < cost(solution);
+      assert false;
+    } 
     else
-    { 
-      while ( 0 < i )
-        invariant  0 <= i <= 4
-        invariant forall index :: 4 >= index >= i ==> optimalSolution[index] <= 1
+    {
+      while (0 < i)
+        invariant 0 <= i <= 4
+        invariant forall index::4 >= index >= i ==> optimalSolution[index] <= 1 
       {
         i:= i - 1;
-        if(optimalSolution[i] > 1)
+        if (optimalSolution[i] > 1) 
         {
-          var solution := optimalSolution[i:=optimalSolution[i]-2];
-          solution :=solution[i+1:=solution[i+1]+1];
+          var solution:= optimalSolution[i:= optimalSolution[i] - 2];
+          solution:= solution[i + 1:= solution[i + 1] + 1];
           assert isSolution(solution, rest - 32);
           assert cost(solution) == cost(optimalSolution) - 1;
           assert cost(optimalSolution) - 1 < cost(solution);
           assert false;
         }
-          assert optimalSolution[i] <= 1;     
+        assert optimalSolution[i] <= 1;
       }
-        assert solutionElementsSum(optimalSolution) <= rest-1;
-        assert isOptimalSolution(solution, rest);
-        assert false; 
+      assert solutionElementsSum(optimalSolution) <= rest - 1;
+      assert isOptimalSolution(solution, rest);
+      assert false;
     }
   }
 }
 
-lemma banknoteMaxim(rest: int, sum: int, finalSolution: seq<int>, index: int)
-  requires 0<=index<=4
-  requires power(2,index) <= rest < power(2,index+1)
+lemma banknoteMaxim(rest: int, sum: int, finalSolution: seq < int > , index: int)
+  requires 0 <= index <= 4
+  requires power(2, index) <= rest < power(2, index + 1)
   requires isValidSolution(finalSolution)
   requires addOptimRestEqualsOptimSum(rest, sum, finalSolution)
-  ensures addOptimRestEqualsOptimSum(rest - power(2,index), sum,finalSolution[index:=finalSolution[index]+1])
+  ensures addOptimRestEqualsOptimSum(rest - power(2, index), sum, finalSolution[index:= finalSolution[index] + 1]) 
 {
-    var banknote:=power(2,index);
-    forall currentSolution | isValidSolution(currentSolution) && isOptimalSolution(currentSolution, rest - banknote)
-        ensures isOptimalSolution(solutionsSum(solutionsSum(currentSolution, finalSolution), [0,0,0,0,0,0][index:=1]), sum)
-    {
-      assert isSolution(currentSolution, rest - banknote);
-      assert isSolution(currentSolution[index:=currentSolution[index]+1], rest);
+  var banknote:= power(2, index);
+  forall currentSolution | isValidSolution(currentSolution) && isOptimalSolution(currentSolution, rest - banknote)
+    ensures isOptimalSolution(solutionsSum(solutionsSum(currentSolution, finalSolution), [0, 0, 0, 0, 0, 0][index:= 1]), sum) 
+  {
+    assert isSolution(currentSolution, rest - banknote);
+    assert isSolution(currentSolution[index:= currentSolution[index] + 1], rest);
 
-      exchangeArgument(rest, currentSolution, index);
+    exchangeArgument(rest, currentSolution, index);
 
-      assert forall solution :: isValidSolution(solution) && isSolution(solution, rest - banknote) ==> cost(solution) >= cost(currentSolution);
-      assert isSolution(solutionsSum(solutionsSum(currentSolution, finalSolution), [0,0,0,0,0,0][index:=1]), sum);
-      assert forall solution :: isValidSolution(solution) && isSolution(solution, sum) ==> cost(solution) >= cost(solutionsSum(solutionsSum(currentSolution, finalSolution), [0,0,0,0,0,0][index:=1]));
-    }
-    assert forall currentSolution :: isValidSolution(currentSolution) && isOptimalSolution(currentSolution, rest - banknote)  ==> isOptimalSolution(solutionsSum(solutionsSum(currentSolution, finalSolution), [0,0,0,0,0,0][index:=1]), sum); 
+    assert forall solution::isValidSolution(solution) && isSolution(solution, rest - banknote) ==> cost(solution) >= cost(currentSolution);
+    assert isSolution(solutionsSum(solutionsSum(currentSolution, finalSolution), [0, 0, 0, 0, 0, 0][index:= 1]), sum);
+    assert forall solution::isValidSolution(solution) && isSolution(solution, sum) ==> cost(solution) >= cost(solutionsSum(solutionsSum(currentSolution, finalSolution), [0, 0, 0, 0, 0, 0][index:= 1]));
+  }
+  assert forall currentSolution::isValidSolution(currentSolution) && isOptimalSolution(currentSolution, rest - banknote) ==> isOptimalSolution(solutionsSum(solutionsSum(currentSolution, finalSolution), [0, 0, 0, 0, 0, 0][index:= 1]), sum);
 }
- 
-lemma currentSolutionAreCostMin(rest: int, sum: int, solution: seq<int>)
+
+lemma currentSolutionAreCostMin(rest: int, sum: int, solution: seq < int > )
   requires isValidSolution(solution)
   requires rest >= 32
   requires isSolution(solution, rest - 32)
   requires isOptimalSolution(solution, rest - 32)
-  ensures isOptimalSolution(solutionsSum(solution, [0,0,0,0,0,1]), rest)
+  ensures isOptimalSolution(solutionsSum(solution, [0, 0, 0, 0, 0, 1]), rest) 
 {
   forall someSolution | isValidSolution(someSolution) && isSolution(someSolution, rest)
-    ensures cost(someSolution) >= cost(solutionsSum(solution, [0,0,0,0,0,1]))
+    ensures cost(someSolution) >= cost(solutionsSum(solution, [0, 0, 0, 0, 0, 1])) 
   {
     exchangeArgument32(rest, sum, someSolution, solution);
-  } 
+  }
 }
 
-lemma banknoteMaxim32(rest: int, sum: int, finalSolution: seq<int>)
+lemma banknoteMaxim32(rest: int, sum: int, finalSolution: seq < int > )
   requires rest >= 32
   requires isValidSolution(finalSolution)
   requires addOptimRestEqualsOptimSum(rest, sum, finalSolution)
-  ensures addOptimRestEqualsOptimSum(rest - 32, sum, solutionsSum(finalSolution, [0,0,0,0,0,1]))
+  ensures addOptimRestEqualsOptimSum(rest - 32, sum, solutionsSum(finalSolution, [0, 0, 0, 0, 0, 1])) 
 {
-   forall currentSolution | isValidSolution(currentSolution) && isSolution(currentSolution, rest - 32) 
-      ensures isSolution(solutionsSum(solutionsSum(finalSolution, currentSolution), [0,0,0,0,0,1]), sum)
-   {
-     assert isSolution(solutionsSum(currentSolution, [0,0,0,0,0,1]), rest);
-   }
-      
-  forall currentSolution | isValidSolution(currentSolution) && isOptimalSolution(currentSolution, rest - 32) 
-      ensures isOptimalSolution(solutionsSum(solutionsSum(finalSolution, currentSolution), [0,0,0,0,0,1]), sum)
+  forall currentSolution | isValidSolution(currentSolution) && isSolution(currentSolution, rest - 32)
+    ensures isSolution(solutionsSum(solutionsSum(finalSolution, currentSolution), [0, 0, 0, 0, 0, 1]), sum) 
+  {
+    assert isSolution(solutionsSum(currentSolution, [0, 0, 0, 0, 0, 1]), rest);
+  }
+
+  forall currentSolution | isValidSolution(currentSolution) && isOptimalSolution(currentSolution, rest - 32)
+    ensures isOptimalSolution(solutionsSum(solutionsSum(finalSolution, currentSolution), [0, 0, 0, 0, 0, 1]), sum)
   {
     assert isSolution(currentSolution, rest - 32);
-    assert isSolution(solutionsSum(currentSolution, [0,0,0,0,0,1]), rest);
-    assert isSolution(solutionsSum(solutionsSum(currentSolution, finalSolution), [0,0,0,0,0,1]), sum);
+    assert isSolution(solutionsSum(currentSolution, [0, 0, 0, 0, 0, 1]), rest);
+    assert isSolution(solutionsSum(solutionsSum(currentSolution, finalSolution), [0, 0, 0, 0, 0, 1]), sum);
 
-    assert forall someSolution :: isValidSolution(someSolution) && isSolution(someSolution, rest - 32) ==> cost(someSolution) >= cost(currentSolution);
-    
+    assert forall someSolution::isValidSolution(someSolution) && isSolution(someSolution, rest - 32) ==> cost(someSolution) >= cost(currentSolution);
+
     forall someSolution | isValidSolution(someSolution) && isSolution(someSolution, sum)
-      ensures cost(someSolution) >= cost(solutionsSum(solutionsSum(finalSolution, currentSolution), [0,0,0,0,0,1]))
+      ensures cost(someSolution) >= cost(solutionsSum(solutionsSum(finalSolution, currentSolution), [0, 0, 0, 0, 0, 1])) 
     {
-        currentSolutionAreCostMin(rest, sum, currentSolution);
+      currentSolutionAreCostMin(rest, sum, currentSolution);
     }
   }
 }
 
-method banknoteMinimum(sum: int) returns (solution: seq<int>)
-  requires sum >= 0 
+method banknoteMinimum(sum: int) returns(solution: seq < int > )
+  requires sum >= 0
   ensures isValidSolution(solution)
   ensures isSolution(solution, sum)
-  ensures isOptimalSolution(solution, sum)
+  ensures isOptimalSolution(solution, sum) 
 {
-   var rest := sum;
-   solution:=[0, 0, 0, 0, 0, 0];
-   var index:=0;
-   assert isOptimalSolution(solution, sum - rest) ;
-   while (0 < rest )
+  var rest:= sum;
+  solution:= [0, 0, 0, 0, 0, 0];
+  var index:= 0;
+  assert isOptimalSolution(solution, sum - rest);
+  while (0 < rest)
     invariant 0 <= rest <= sum
-    invariant |solution|==6
-    invariant forall i :: 0<=i<=5 ==> solution[i]>=0
+    invariant isValidSolution(solution)
     invariant isSolution(solution, sum - rest)
     invariant addOptimRestEqualsOptimSum(rest, sum, solution)
-    decreases rest
-  {
-    //at every iteration it chooses the banknote optimal for rest, then modifies solution
-    index:=maxBanknote(rest);
-    var banknote:=power(2,index);
-    if(index!=5)
+    decreases rest 
     {
-      banknoteMaxim(rest, sum, solution,index);
-     }
-    else 
-    {
-      banknoteMaxim32(rest, sum, solution);
-    }
-    assert isSolution(solution[index:=solution[index]+1], sum - rest + banknote); 
-    assert addOptimRestEqualsOptimSum(rest - banknote, sum, solution[index:=solution[index]+1]);
-    solution := solution[index:=solution[index]+1];
-    rest := rest - banknote; 
+      //at every iteration it chooses the banknote optimal for rest, then modifies solution
+      index:= maxBanknote(rest);
+      var banknote:= power(2, index);
+      if (index != 5) 
+      {
+        banknoteMaxim(rest, sum, solution, index);
+      } 
+       else 
+      {
+        banknoteMaxim32(rest, sum, solution);
+      }
+      assert isSolution(addValueToIndex(solution,1,index), sum - rest + banknote);
+      assert addOptimRestEqualsOptimSum(rest - banknote, sum, addValueToIndex(solution,1,index));
+      solution:= addValueToIndex(solution,1,index);
+      rest:= rest - banknote;
   }
 }
 
-method Main () 
-{
-  var sum := 81;
-  var solution := banknoteMinimum(sum);
+method Main() {
+  var sum:= 81;
+  var solution:= banknoteMinimum(sum);
   print "Optimum change for ";
   print sum;
   print " is: ";
@@ -321,5 +326,5 @@ method Main ()
   print " \n Banknotes of 16: ";
   print solution[4];
   print "\n Banknotes of 32: ";
-  print solution[5]; 
+  print solution[5];
 }
